@prefix : <http://www.semanticweb.org/usuario/ontologies/2024/3/untitled-ontology-5/> .
@prefix owl: <http://www.w3.org/2002/07/owl#> .
@prefix rdf: <http://www.w3.org/1999/02/22-rdf-syntax-ns#> .
@prefix xml: <http://www.w3.org/XML/1998/namespace> .
@prefix xsd: <http://www.w3.org/2001/XMLSchema#> .
@prefix rdfs: <http://www.w3.org/2000/01/rdf-schema#> .
@base <http://www.semanticweb.org/usuario/ontologies/2024/3/untitled-ontology-5/> .

<http://www.semanticweb.org/usuario/ontologies/2024/3/untitled-ontology-5> rdf:type owl:Ontology .

#################################################################
#    Object Properties
#################################################################

###  http://www.semanticweb.org/usuario/ontologies/2024/3/untitled-ontology-5/fliesOn
:fliesOn rdf:type owl:ObjectProperty ;
         rdfs:subPropertyOf owl:topObjectProperty ;
         rdfs:domain :Passenger ;
         rdfs:range :Flight ;
         rdfs:comment "Associates a passenger with a specific flight they have taken. This property helps in tracking the flights on which a passenger was a traveler, providing a direct connection between the individual and the flight details." ;
         rdfs:label "Flies On" .


###  http://www.semanticweb.org/usuario/ontologies/2024/3/untitled-ontology-5/hasReview
:hasReview rdf:type owl:ObjectProperty ;
           rdfs:subPropertyOf owl:topObjectProperty ;
           rdfs:domain :Passenger ;
           rdfs:range :Review ;
           rdfs:comment "Connects a passenger to a review they have authored. This property links the passenger who wrote the review with the actual feedback provided." ;
           rdfs:label "Has Review" .


###  http://www.semanticweb.org/usuario/ontologies/2024/3/untitled-ontology-5/reviewOfFlight
:reviewOfFlight rdf:type owl:ObjectProperty ;
                rdfs:subPropertyOf owl:topObjectProperty ;
                rdfs:domain :Review ;
                rdfs:range :Flight ;
                rdfs:comment "Links to a review of the flight it belongs to.This property associates a specific review with the corresponding flight, which will allow detailed analysis of passenger experiences based on individual flights." ;
                rdfs:label "Review of Flight" .


#################################################################
#    Data properties
#################################################################

###  http://www.semanticweb.org/usuario/ontologies/2024/3/untitled-ontology-5#Food_&_Beverages
<http://www.semanticweb.org/usuario/ontologies/2024/3/untitled-ontology-5#Food_&_Beverages> rdf:type owl:DatatypeProperty ;
                                                                                            rdfs:subPropertyOf owl:topDataProperty ;
                                                                                            rdfs:domain <http://www.semanticweb.org/usuario/ontologies/2024/3/untitled-ontology-5#Food_&_Beverages> ;
                                                                                            rdfs:range xsd:decimal .


###  http://www.semanticweb.org/usuario/ontologies/2024/3/untitled-ontology-5#Food_&_Beverages:_Name
<http://www.semanticweb.org/usuario/ontologies/2024/3/untitled-ontology-5#Food_&_Beverages:_Name> rdf:type owl:DatatypeProperty ;
                                                                                                  rdfs:subPropertyOf owl:topDataProperty ;
                                                                                                  rdfs:domain <http://www.semanticweb.org/usuario/ontologies/2024/3/untitled-ontology-5#Food_&_Beverages> ;
                                                                                                  rdfs:range xsd:string ;
                                                                                                  rdfs:comment "Indicates the name of the foods and beverages that the passenger drinks and eats." ;
                                                                                                  rdfs:label "Name of the Food & Beverages" .


###  http://www.semanticweb.org/usuario/ontologies/2024/3/untitled-ontology-5#Wifi_&_Connectivity
<http://www.semanticweb.org/usuario/ontologies/2024/3/untitled-ontology-5#Wifi_&_Connectivity> rdf:type owl:DatatypeProperty ;
                                                                                               rdfs:subPropertyOf owl:topDataProperty .


###  http://www.semanticweb.org/usuario/ontologies/2024/3/untitled-ontology-5/Cabin_Staff_Service
:Cabin_Staff_Service rdf:type owl:DatatypeProperty ;
                     rdfs:subPropertyOf owl:topDataProperty ;
                     rdfs:domain :Cabin_Staff_Service ;
                     rdfs:range xsd:decimal .


###  http://www.semanticweb.org/usuario/ontologies/2024/3/untitled-ontology-5/Country
:Country rdf:type owl:DatatypeProperty ;
         rdfs:subPropertyOf owl:topDataProperty ;
         rdfs:domain :Country ;
         rdfs:range xsd:string .


###  http://www.semanticweb.org/usuario/ontologies/2024/3/untitled-ontology-5/Date_Flown
:Date_Flown rdf:type owl:DatatypeProperty ;
            rdfs:subPropertyOf owl:topDataProperty ;
            rdfs:domain :Flight ;
            rdfs:range xsd:string .


###  http://www.semanticweb.org/usuario/ontologies/2024/3/untitled-ontology-5/Destination
:Destination rdf:type owl:DatatypeProperty ;
             rdfs:subPropertyOf owl:topDataProperty ;
             rdfs:domain :Flight ;
             rdfs:range xsd:string .


###  http://www.semanticweb.org/usuario/ontologies/2024/3/untitled-ontology-5/Overall_Rating
:Overall_Rating rdf:type owl:DatatypeProperty ;
                rdfs:subPropertyOf owl:topDataProperty ;
                rdfs:domain :Flight ;
                rdfs:range xsd:integer .


###  http://www.semanticweb.org/usuario/ontologies/2024/3/untitled-ontology-5/Recommended
:Recommended rdf:type owl:DatatypeProperty ;
             rdfs:subPropertyOf owl:topDataProperty ;
             rdfs:domain :Recommended ;
             rdfs:range xsd:boolean .


###  http://www.semanticweb.org/usuario/ontologies/2024/3/untitled-ontology-5/Seat_Comfort
:Seat_Comfort rdf:type owl:DatatypeProperty ;
              rdfs:subPropertyOf owl:topDataProperty ;
              rdfs:domain :Seat_Comfort ;
              rdfs:range xsd:decimal .


###  http://www.semanticweb.org/usuario/ontologies/2024/3/untitled-ontology-5/Trip_verified
:Trip_verified rdf:type owl:DatatypeProperty ;
               rdfs:subPropertyOf owl:topDataProperty ;
               rdfs:domain :Flight ;
               rdfs:range xsd:string .


###  http://www.semanticweb.org/usuario/ontologies/2024/3/untitled-ontology-5/flightNumber
:flightNumber rdf:type owl:DatatypeProperty ;
              rdfs:subPropertyOf owl:topDataProperty ;
              rdfs:domain :Flight ;
              rdfs:range xsd:string ;
              rdfs:comment "Identifies the specific flight by its unique alphanumeric code." ;
              rdfs:label "Flight Number" .


###  http://www.semanticweb.org/usuario/ontologies/2024/3/untitled-ontology-5/reviewDate
:reviewDate rdf:type owl:DatatypeProperty ;
            rdfs:subPropertyOf owl:topDataProperty ;
            rdfs:domain :Review ;
            rdfs:range xsd:dateTime ;
            rdfs:comment "The date on which the review was posted by the passenger." ;
            rdfs:label "Review Date" .


###  http://www.semanticweb.org/usuario/ontologies/2024/3/untitled-ontology-5/reviewRating
:reviewRating rdf:type owl:DatatypeProperty ;
              rdfs:subPropertyOf owl:topDataProperty ;
              rdfs:domain :Review ;
              rdfs:range xsd:integer ;
              rdfs:comment "A numeric value given by a passenger to rate their overall satisfaction with the flight. This rating is typically on a scale from 1 to 10, where 10 represents the highest level of satisfaction." ;
              rdfs:label "Review Rating" .


###  http://www.w3.org/2002/07/owl#topDataProperty
owl:topDataProperty rdfs:domain <http://www.semanticweb.org/usuario/ontologies/2024/3/untitled-ontology-5#Wifi_&_Connectivity> ;
                    rdfs:range xsd:decimal .


#################################################################
#    Classes
#################################################################

###  http://www.semanticweb.org/usuario/ontologies/2024/3/untitled-ontology-5#FrequentDelayVictim
:FrequentDelayVictim rdf:type owl:Class ;
                     rdfs:subClassOf :Passenger ;
                     rdfs:comment "Identifies individuals who have frequently experienced delayed flights. This class is used to categorize passengers based on their unfortunate consistent experience with delays, allowing for targeted customer service interventions such as compensations or personalized communications." ;
                     rdfs:label "Frequent Delay Victim" .


###  http://www.semanticweb.org/usuario/ontologies/2024/3/untitled-ontology-5#RequiresAttention
:RequiresAttention rdf:type owl:Class ;
                   rdfs:subClassOf :Flight ;
                   rdfs:comment "Identify if a flight needs special attention due to negative reviews or other operational concerns. This classification helps prioritize flights for review and intervention by the airline's operational." ;
                   rdfs:label "Requires Attention" .


###  http://www.semanticweb.org/usuario/ontologies/2024/3/untitled-ontology-5#Food_&_Beverages
<http://www.semanticweb.org/usuario/ontologies/2024/3/untitled-ontology-5#Food_&_Beverages> rdf:type owl:Class ;
                                                                                            rdfs:subClassOf :Service .


###  http://www.semanticweb.org/usuario/ontologies/2024/3/untitled-ontology-5#Wifi_&_Connectivity
<http://www.semanticweb.org/usuario/ontologies/2024/3/untitled-ontology-5#Wifi_&_Connectivity> rdf:type owl:Class ;
                                                                                               rdfs:subClassOf :Service .


###  http://www.semanticweb.org/usuario/ontologies/2024/3/untitled-ontology-5/Aircraft
:Aircraft rdf:type owl:Class ;
          rdfs:subClassOf :Flight ;
          rdfs:comment "Specifies the model of aircraft used for the flight." ;
          rdfs:label "Aircraft" .


###  http://www.semanticweb.org/usuario/ontologies/2024/3/untitled-ontology-5/Airline
:Airline rdf:type owl:Class ;
         rdfs:comment "Represents an airline company that operates flights. This class can include properties that describe the airline, such as its verification status, etc." ;
         rdfs:label "Airline" .


###  http://www.semanticweb.org/usuario/ontologies/2024/3/untitled-ontology-5/Cabin_Staff_Service
:Cabin_Staff_Service rdf:type owl:Class ;
                     rdfs:subClassOf :Service .


###  http://www.semanticweb.org/usuario/ontologies/2024/3/untitled-ontology-5/Comment
:Comment rdf:type owl:Class ;
         rdfs:subClassOf :Review ;
         rdfs:comment "A detailed comment about the flight experience." ;
         rdfs:label "Comment" .


###  http://www.semanticweb.org/usuario/ontologies/2024/3/untitled-ontology-5/Comment_title
:Comment_title rdf:type owl:Class ;
               rdfs:subClassOf :Review ;
               rdfs:comment "A brief headline for the comment provided by the passenger, summarizing the essence of their feedback." ;
               rdfs:label "Comment Title" .


###  http://www.semanticweb.org/usuario/ontologies/2024/3/untitled-ontology-5/Country
:Country rdf:type owl:Class ;
         rdfs:subClassOf :Passenger .


###  http://www.semanticweb.org/usuario/ontologies/2024/3/untitled-ontology-5/Date_Flown
:Date_Flown rdf:type owl:Class ;
            rdfs:subClassOf :Flight .


###  http://www.semanticweb.org/usuario/ontologies/2024/3/untitled-ontology-5/Date_Published
:Date_Published rdf:type owl:Class ;
                rdfs:subClassOf :Review ;
                rdfs:comment "The date on which the review was published." ;
                rdfs:label "Date Published" .


###  http://www.semanticweb.org/usuario/ontologies/2024/3/untitled-ontology-5/Destination
:Destination rdf:type owl:Class ;
             rdfs:subClassOf :Flight .


###  http://www.semanticweb.org/usuario/ontologies/2024/3/untitled-ontology-5/Flight
:Flight rdf:type owl:Class ;
        rdfs:comment "Represents an instance of an airline flight, containing details about the flight's origin, destination, date flown and the aircraft." ;
        rdfs:label "Flight" .


###  http://www.semanticweb.org/usuario/ontologies/2024/3/untitled-ontology-5/Ground_Service
:Ground_Service rdf:type owl:Class ;
                rdfs:subClassOf :Service ;
                rdfs:comment "Evaluates the efficiency and quality of airport ground services." ;
                rdfs:label "Ground Service" .


###  http://www.semanticweb.org/usuario/ontologies/2024/3/untitled-ontology-5/Inflight_Entertainment
:Inflight_Entertainment rdf:type owl:Class ;
                        rdfs:subClassOf :Service ;
                        rdfs:comment "Assesses the quality and variety of entertainment options available during the flight." ;
                        rdfs:label "Inflight Entertainment" .


###  http://www.semanticweb.org/usuario/ontologies/2024/3/untitled-ontology-5/Max_Rating
:Max_Rating rdf:type owl:Class ;
            rdfs:subClassOf :Review ;
            rdfs:comment "The highest possible rating on the review scale." ;
            rdfs:label "Max Rating" .


###  http://www.semanticweb.org/usuario/ontologies/2024/3/untitled-ontology-5/Origin
:Origin rdf:type owl:Class ;
        rdfs:subClassOf :Flight ;
        rdfs:comment "The departure location of the flight." ;
        rdfs:label "Origin" .


###  http://www.semanticweb.org/usuario/ontologies/2024/3/untitled-ontology-5/Overall_Rating
:Overall_Rating rdf:type owl:Class ;
                rdfs:subClassOf :Review .


###  http://www.semanticweb.org/usuario/ontologies/2024/3/untitled-ontology-5/Passenger
:Passenger rdf:type owl:Class ;
           rdfs:subClassOf [ rdf:type owl:Restriction ;
                             owl:onProperty :fliesOn ;
                             owl:minQualifiedCardinality "1"^^xsd:nonNegativeInteger ;
                             owl:onClass :Flight
                           ] ,
                           [ rdf:type owl:Restriction ;
                             owl:onProperty :hasReview ;
                             owl:minQualifiedCardinality "1"^^xsd:nonNegativeInteger ;
                             owl:onClass :Review
                           ] ;
           rdfs:comment "Represents a person who travels on a plane. Attributes may include the type of traveller and their country of origin." ;
           rdfs:label "Passenger" .


###  http://www.semanticweb.org/usuario/ontologies/2024/3/untitled-ontology-5/Passenger_Country
:Passenger_Country rdf:type owl:Class ;
                   rdfs:subClassOf :Passenger ;
                   rdfs:comment "The country of origin/birth of the passenger." ;
                   rdfs:label "Passenger Country" .


###  http://www.semanticweb.org/usuario/ontologies/2024/3/untitled-ontology-5/Rating
:Rating rdf:type owl:Class ;
        rdfs:subClassOf :Review ;
        rdfs:comment "A numerical rating given by the passenger for the overall flight experience." ;
        rdfs:label "Rating" .


###  http://www.semanticweb.org/usuario/ontologies/2024/3/untitled-ontology-5/Recommended
:Recommended rdf:type owl:Class ;
             rdfs:subClassOf :Review .


###  http://www.semanticweb.org/usuario/ontologies/2024/3/untitled-ontology-5/Review
:Review rdf:type owl:Class ;
        rdfs:comment "Contains information about a passenger's review of a flight. This includes ratings, comments, and publication details." ;
        rdfs:label "Review" .


###  http://www.semanticweb.org/usuario/ontologies/2024/3/untitled-ontology-5/Review_Body
:Review_Body rdf:type owl:Class ;
             rdfs:subClassOf :Review ;
             rdfs:comment "The main content of the review, where the passenger details their full experience and observations about the flight." ;
             rdfs:label "Review Body" .


###  http://www.semanticweb.org/usuario/ontologies/2024/3/untitled-ontology-5/Seat_Comfort
:Seat_Comfort rdf:type owl:Class ;
              rdfs:subClassOf :Service .


###  http://www.semanticweb.org/usuario/ontologies/2024/3/untitled-ontology-5/Seat_Type
:Seat_Type rdf:type owl:Class ;
           rdfs:subClassOf :Service ;
           rdfs:comment "The type of seat the passenger had during the flight, e.g., economy, business." ;
           rdfs:label "Seat Type" .


###  http://www.semanticweb.org/usuario/ontologies/2024/3/untitled-ontology-5/Service
:Service rdf:type owl:Class ;
         rdfs:comment "Represents various aspects of service provided during the flight, rated by passengers." ;
         rdfs:label "Service" .


###  http://www.semanticweb.org/usuario/ontologies/2024/3/untitled-ontology-5/Title
:Title rdf:type owl:Class ;
       rdfs:subClassOf :Review ;
       rdfs:comment "The title of the review provided by the passenger." ;
       rdfs:label "Title" .


###  http://www.semanticweb.org/usuario/ontologies/2024/3/untitled-ontology-5/Trip_verified
:Trip_verified rdf:type owl:Class ;
               rdfs:subClassOf :Airline .


###  http://www.semanticweb.org/usuario/ontologies/2024/3/untitled-ontology-5/Type_Of_Traveller
:Type_Of_Traveller rdf:type owl:Class ;
                   rdfs:subClassOf :Passenger ;
                   rdfs:comment "Describes the travel context of the passenger, such as business or leisure." ;
                   rdfs:label "Type of Traveller" .


###  http://www.semanticweb.org/usuario/ontologies/2024/3/untitled-ontology-5/Value_For_Money
:Value_For_Money rdf:type owl:Class ;
                 rdfs:subClassOf :Service ;
                 rdfs:comment "The passenger's assessment of the overall value for the cost of the flight." ;
                 rdfs:label "Value for Money" .


###  http://www.semanticweb.org/usuario/ontologies/2024/3/untitled-ontology-5/Verified
:Verified rdf:type owl:Class ;
          rdfs:subClassOf :Airline ;
          rdfs:comment "Indicates whether the airline's profile has been officially verified." ;
          rdfs:label "Verified" .


#################################################################
#    Individuals
#################################################################

###  http://www.semanticweb.org/usuario/ontologies/2024/3/untitled-ontology-5/Eugene_Tan
:Eugene_Tan rdf:type owl:NamedIndividual ,
                     :Passenger ;
            :fliesOn :FlightQA001 ;
            :hasReview :Review001 ;
            :reviewOfFlight :FlightQA001 ;
            <http://www.semanticweb.org/usuario/ontologies/2024/3/untitled-ontology-5#Food_&_Beverages> 5.0 ;
            <http://www.semanticweb.org/usuario/ontologies/2024/3/untitled-ontology-5#Food_&_Beverages:_Name> "Salad and orange juice" ;
            <http://www.semanticweb.org/usuario/ontologies/2024/3/untitled-ontology-5#Wifi_&_Connectivity> 2.0 ;
            :Cabin_Staff_Service 3.0 ;
            :Country "Lisbon" ;
            :Date_Flown "03-01-2024"^^xsd:dateTime ;
            :Destination "Manchester" ;
            :Overall_Rating 9 ;
            :Recommended "false"^^xsd:boolean ;
            :Seat_Comfort 3.0 ;
            :Trip_verified "Not Verified" ;
            :flightNumber "FlightQA003" .


###  http://www.semanticweb.org/usuario/ontologies/2024/3/untitled-ontology-5/FlightQA001
:FlightQA001 rdf:type owl:NamedIndividual ,
                      :Flight ;
             :Date_Flown "March 2024" ;
             :Destination "London Heathrow via Doha" ;
             :flightNumber 777 ;
             :reviewDate "02-03-2024"^^xsd:dateTime .


###  http://www.semanticweb.org/usuario/ontologies/2024/3/untitled-ontology-5/FoodBeverages001
:FoodBeverages001 rdf:type owl:NamedIndividual ,
                           <http://www.semanticweb.org/usuario/ontologies/2024/3/untitled-ontology-5#Food_&_Beverages> ;
                  :reviewOfFlight :FoodBeverages001 ;
                  <http://www.semanticweb.org/usuario/ontologies/2024/3/untitled-ontology-5#Food_&_Beverages> 4.0 ;
                  <http://www.semanticweb.org/usuario/ontologies/2024/3/untitled-ontology-5#Food_&_Beverages:_Name> "Pasta, chicken and water" .


###  http://www.semanticweb.org/usuario/ontologies/2024/3/untitled-ontology-5/Review001
:Review001 rdf:type owl:NamedIndividual ,
                    :Review ;
           <http://www.semanticweb.org/usuario/ontologies/2024/3/untitled-ontology-5#Food_&_Beverages:_Name> "Fish and water" ;
           <http://www.semanticweb.org/usuario/ontologies/2024/3/untitled-ontology-5#Wifi_&_Connectivity> 1.0 ;
           :Cabin_Staff_Service 3.0 ;
           :Country "Spain" ;
           :Destination "United States" ;
           :Overall_Rating 2.0 ;
           :Recommended "false"^^xsd:boolean ;
           :Seat_Comfort 2.0 ;
           :Trip_verified "Trip Verified" ;
           :flightNumber "FlightQA004" ;
           :reviewDate "01-01-2023"^^xsd:dateTime ;
           :reviewRating 4.0 .


###  http://www.semanticweb.org/usuario/ontologies/2024/3/untitled-ontology-5/Wayne_Burgess
:Wayne_Burgess rdf:type owl:NamedIndividual ,
                        :Passenger ;
               :fliesOn :FlightQA001 ;
               :hasReview :Review001 ;
               :Country "United Kingdom" ;
               :Date_Flown "October 2023" ;
               :Destination "Paris Beauvais" ;
               :flightNumber "FlightQA002" ;
               :reviewDate "29-02-2024"^^xsd:dateTime ;
               :reviewRating 1 .


#################################################################
#    Annotations
#################################################################

<http://www.semanticweb.org/usuario/ontologies/2024/3/untitled-ontology-5#Food_&_Beverages> rdfs:comment "Rate the quality of food and beverages that the passenger drinks and eats." ;
                                                                                            rdfs:label "Food & Beverages" .


<http://www.semanticweb.org/usuario/ontologies/2024/3/untitled-ontology-5#Wifi_&_Connectivity> rdfs:comment "Evaluates the availability and quality of WiFi and other connectivity options on board." ;
                                                                                               rdfs:label "WiFi & Connectivity" .


:Cabin_Staff_Service rdfs:comment "Reflects on the performance and friendliness of the cabin crew." ;
                     rdfs:label "Cabin Staff Service" .


:Country rdfs:comment "The country where the passenger resides, which may influence their travel preferences and perspectives." ;
         rdfs:label "Country of residence" .


:Date_Flown rdfs:comment "The date on which the flight took place." ;
            rdfs:label "Date Flown" .


:Destination rdfs:comment "Destination" ,
                          "The arrival location of the flight." .


:Overall_Rating rdfs:comment "An aggregate score reflecting the total satisfaction level of the passenger." ;
                rdfs:label "Overall Rating" .


:Recommended rdfs:comment "Indicates whether the passenger would recommend the airline to others." ;
             rdfs:label "Recommended" .


:Seat_Comfort rdfs:comment "Describes the comfort level of the airplane seating." ;
              rdfs:label "Seat Comfort" .


:Trip_verified rdfs:comment "Indicates whether the details of the flight have been verified as part of a review process, ensuring the authenticity of the information provided." ;
               rdfs:label "Trip Verified" .


#################################################################
#    Rules
#################################################################

<urn:swrl:var#f> rdf:type <http://www.w3.org/2003/11/swrl#Variable> .

<urn:swrl:var#r> rdf:type <http://www.w3.org/2003/11/swrl#Variable> .

<urn:swrl:var#rating> rdf:type <http://www.w3.org/2003/11/swrl#Variable> .

<urn:swrl:var#r1> rdf:type <http://www.w3.org/2003/11/swrl#Variable> .

<urn:swrl:var#rating1> rdf:type <http://www.w3.org/2003/11/swrl#Variable> .

<urn:swrl:var#r2> rdf:type <http://www.w3.org/2003/11/swrl#Variable> .

<urn:swrl:var#rating2> rdf:type <http://www.w3.org/2003/11/swrl#Variable> .

[ rdf:type <http://www.w3.org/2003/11/swrl#Imp> ;
   <http://www.w3.org/2003/11/swrl#body> [ rdf:type <http://www.w3.org/2003/11/swrl#AtomList> ;
                                           rdf:first [ rdf:type <http://www.w3.org/2003/11/swrl#ClassAtom> ;
                                                       <http://www.w3.org/2003/11/swrl#classPredicate> :Flight ;
                                                       <http://www.w3.org/2003/11/swrl#argument1> <urn:swrl:var#f>
                                                     ] ;
                                           rdf:rest [ rdf:type <http://www.w3.org/2003/11/swrl#AtomList> ;
                                                      rdf:first [ rdf:type <http://www.w3.org/2003/11/swrl#IndividualPropertyAtom> ;
                                                                  <http://www.w3.org/2003/11/swrl#propertyPredicate> :hasReview ;
                                                                  <http://www.w3.org/2003/11/swrl#argument1> <urn:swrl:var#f> ;
                                                                  <http://www.w3.org/2003/11/swrl#argument2> <urn:swrl:var#r1>
                                                                ] ;
                                                      rdf:rest [ rdf:type <http://www.w3.org/2003/11/swrl#AtomList> ;
                                                                 rdf:first [ rdf:type <http://www.w3.org/2003/11/swrl#DatavaluedPropertyAtom> ;
                                                                             <http://www.w3.org/2003/11/swrl#propertyPredicate> :reviewRating ;
                                                                             <http://www.w3.org/2003/11/swrl#argument1> <urn:swrl:var#r1> ;
                                                                             <http://www.w3.org/2003/11/swrl#argument2> <urn:swrl:var#rating1>
                                                                           ] ;
                                                                 rdf:rest [ rdf:type <http://www.w3.org/2003/11/swrl#AtomList> ;
                                                                            rdf:first [ rdf:type <http://www.w3.org/2003/11/swrl#BuiltinAtom> ;
                                                                                        <http://www.w3.org/2003/11/swrl#builtin> <http://www.w3.org/2003/11/swrlb#lessThan> ;
                                                                                        <http://www.w3.org/2003/11/swrl#arguments> [ rdf:type rdf:List ;
                                                                                                                                     rdf:first <urn:swrl:var#rating1> ;
                                                                                                                                     rdf:rest [ rdf:type rdf:List ;
                                                                                                                                                rdf:first 3 ;
                                                                                                                                                rdf:rest rdf:nil
                                                                                                                                              ]
                                                                                                                                   ]
                                                                                      ] ;
                                                                            rdf:rest [ rdf:type <http://www.w3.org/2003/11/swrl#AtomList> ;
                                                                                       rdf:first [ rdf:type <http://www.w3.org/2003/11/swrl#IndividualPropertyAtom> ;
                                                                                                   <http://www.w3.org/2003/11/swrl#propertyPredicate> :hasReview ;
                                                                                                   <http://www.w3.org/2003/11/swrl#argument1> <urn:swrl:var#f> ;
                                                                                                   <http://www.w3.org/2003/11/swrl#argument2> <urn:swrl:var#r2>
                                                                                                 ] ;
                                                                                       rdf:rest [ rdf:type <http://www.w3.org/2003/11/swrl#AtomList> ;
                                                                                                  rdf:first [ rdf:type <http://www.w3.org/2003/11/swrl#DatavaluedPropertyAtom> ;
                                                                                                              <http://www.w3.org/2003/11/swrl#propertyPredicate> :reviewRating ;
                                                                                                              <http://www.w3.org/2003/11/swrl#argument1> <urn:swrl:var#r2> ;
                                                                                                              <http://www.w3.org/2003/11/swrl#argument2> <urn:swrl:var#rating2>
                                                                                                            ] ;
                                                                                                  rdf:rest [ rdf:type <http://www.w3.org/2003/11/swrl#AtomList> ;
                                                                                                             rdf:first [ rdf:type <http://www.w3.org/2003/11/swrl#BuiltinAtom> ;
                                                                                                                         <http://www.w3.org/2003/11/swrl#builtin> <http://www.w3.org/2003/11/swrlb#lessThan> ;
                                                                                                                         <http://www.w3.org/2003/11/swrl#arguments> [ rdf:type rdf:List ;
                                                                                                                                                                      rdf:first <urn:swrl:var#rating2> ;
                                                                                                                                                                      rdf:rest [ rdf:type rdf:List ;
                                                                                                                                                                                 rdf:first 3 ;
                                                                                                                                                                                 rdf:rest rdf:nil
                                                                                                                                                                               ]
                                                                                                                                                                    ]
                                                                                                                       ] ;
                                                                                                             rdf:rest rdf:nil
                                                                                                           ]
                                                                                                ]
                                                                                     ]
                                                                          ]
                                                               ]
                                                    ]
                                         ] ;
   <http://www.w3.org/2003/11/swrl#head> [ rdf:type <http://www.w3.org/2003/11/swrl#AtomList> ;
                                           rdf:first [ rdf:type <http://www.w3.org/2003/11/swrl#ClassAtom> ;
                                                       <http://www.w3.org/2003/11/swrl#classPredicate> :RequiresAttention ;
                                                       <http://www.w3.org/2003/11/swrl#argument1> <urn:swrl:var#f>
                                                     ] ;
                                           rdf:rest rdf:nil
                                         ]
 ] .

[ rdf:type <http://www.w3.org/2003/11/swrl#Imp> ;
   <http://www.w3.org/2003/11/swrl#body> [ rdf:type <http://www.w3.org/2003/11/swrl#AtomList> ;
                                           rdf:first [ rdf:type <http://www.w3.org/2003/11/swrl#ClassAtom> ;
                                                       <http://www.w3.org/2003/11/swrl#classPredicate> :Flight ;
                                                       <http://www.w3.org/2003/11/swrl#argument1> <urn:swrl:var#f>
                                                     ] ;
                                           rdf:rest [ rdf:type <http://www.w3.org/2003/11/swrl#AtomList> ;
                                                      rdf:first [ rdf:type <http://www.w3.org/2003/11/swrl#IndividualPropertyAtom> ;
                                                                  <http://www.w3.org/2003/11/swrl#propertyPredicate> :hasReview ;
                                                                  <http://www.w3.org/2003/11/swrl#argument1> <urn:swrl:var#f> ;
                                                                  <http://www.w3.org/2003/11/swrl#argument2> <urn:swrl:var#r>
                                                                ] ;
                                                      rdf:rest [ rdf:type <http://www.w3.org/2003/11/swrl#AtomList> ;
                                                                 rdf:first [ rdf:type <http://www.w3.org/2003/11/swrl#DatavaluedPropertyAtom> ;
                                                                             <http://www.w3.org/2003/11/swrl#propertyPredicate> :reviewRating ;
                                                                             <http://www.w3.org/2003/11/swrl#argument1> <urn:swrl:var#r> ;
                                                                             <http://www.w3.org/2003/11/swrl#argument2> <urn:swrl:var#rating>
                                                                           ] ;
                                                                 rdf:rest [ rdf:type <http://www.w3.org/2003/11/swrl#AtomList> ;
                                                                            rdf:first [ rdf:type <http://www.w3.org/2003/11/swrl#BuiltinAtom> ;
                                                                                        <http://www.w3.org/2003/11/swrl#builtin> <http://www.w3.org/2003/11/swrlb#greaterThanOrEqual> ;
                                                                                        <http://www.w3.org/2003/11/swrl#arguments> [ rdf:type rdf:List ;
                                                                                                                                     rdf:first <urn:swrl:var#rating> ;
                                                                                                                                     rdf:rest [ rdf:type rdf:List ;
                                                                                                                                                rdf:first 3 ;
                                                                                                                                                rdf:rest rdf:nil
                                                                                                                                              ]
                                                                                                                                   ]
                                                                                      ] ;
                                                                            rdf:rest rdf:nil
                                                                          ]
                                                               ]
                                                    ]
                                         ] ;
   <http://www.w3.org/2003/11/swrl#head> [ rdf:type <http://www.w3.org/2003/11/swrl#AtomList> ;
                                           rdf:first [ rdf:type <http://www.w3.org/2003/11/swrl#ClassAtom> ;
                                                       <http://www.w3.org/2003/11/swrl#classPredicate> :Recommended ;
                                                       <http://www.w3.org/2003/11/swrl#argument1> <urn:swrl:var#f>
                                                     ] ;
                                           rdf:rest rdf:nil
                                         ]
 ] .

###  Generated by the OWL API (version 4.5.26.2023-07-17T20:34:13Z) https://github.com/owlcs/owlapi
